Iterator/Wrapper.lean
@@ -7,39 +7,41 @@ prelude
 import Iterator.Basic
 import Iterator.Cont
 
-structure Iter {α} (m β) [Iterator α m β] where
-  inner : Iterator.α' α m
+structure Iter {α α'} (m β) [Iterator α α' m β] where
+  inner : α
 
-def Iter.Relations.yielded {α m β} [Iterator α m β] (it it' : Iter (α := α) m β) (output : β) : Prop :=
-  Iterator.yielded it.inner it'.inner (Iterator.βEquiv.hom output)
+variable {α : Type w} {α' : Type u} {m : Type w → Type w'} {β : Type v}
 
-def Iter.Relations.skipped {α m β} [Iterator α m β] (it it' : Iter (α := α) m β) : Prop :=
-  Iterator.skipped it.inner it'.inner
+def Iter.Relations.yielded [Iterator α α' m β] (it it' : Iter (α := α) m β) (output : β) : Prop :=
+  Iterator.yielded (m := m) it.inner it'.inner (Iterator.βEquiv.hom output)
 
-def Iter.Relations.done {α m β} [Iterator α m β] (it : Iter (α := α) m β) : Prop :=
-  Iterator.done it.inner
+def Iter.Relations.skipped [Iterator α α' m β] (it it' : Iter (α := α) m β) : Prop :=
+  Iterator.skipped m it.inner it'.inner
 
-structure Iter.EncodedStep {α m β} [Iterator α m β] (it : Iter (α := α) m β) where
+def Iter.Relations.done [Iterator α α' m β] (it : Iter (α := α) m β) : Prop :=
+  Iterator.done m it.inner
+
+structure Iter.EncodedStep [Iterator α α' m β] (it : Iter (α := α) m β) where
   inner : IterStep.for m it.inner
 
-inductive Iter.Step {α m β} [Iterator α m β] (it : Iter (α := α) m β) where
+inductive Iter.Step [Iterator α α' m β] (it : Iter (α := α) m β) where
   | yield : (it' : Iter (α := α) m β) → (output : β) → Iter.Relations.yielded it it' output → it.Step
   | skip : (it' : Iter (α := α) m β) → Iter.Relations.skipped it it' → it.Step
   | done : Iter.Relations.done it → it.Step
 
 @[always_inline, inline]
-def Iter.EncodedStep.decode {α m β} [Iterator α m β] {it : Iter (α := α) m β} (step : it.EncodedStep) : it.Step :=
+def Iter.EncodedStep.decode [Iterator α α' m β] {it : Iter (α := α) m β} (step : it.EncodedStep) : it.Step :=
   match step.inner with
   | .yield it' out h => .yield ⟨it'⟩ (Iterator.βEquiv.inv out) (by simp [Relations.yielded, Equiv.hom_inv, h])
   | .skip it' h => .skip ⟨it'⟩ h
   | .done h => .done h
 
 @[always_inline, inline]
-def Iter.EncodedStep.ofInternal {α m β} [Iterator α m β] {it : Iter (α := α) m β} (step : IterStep.for m it.inner) : it.EncodedStep :=
+def Iter.EncodedStep.ofInternal [Iterator α α' m β] {it : Iter (α := α) m β} (step : IterStep.for m it.inner) : it.EncodedStep :=
   ⟨step⟩
 
 @[always_inline, inline]
-def toIter (m) [Iterator α m β] (it : Iterator.α' α m) : Iter (α := α) m β :=
+def toIter (m) [Iterator α α' m β] (it : α) : Iter (α := α) m β :=
   ⟨it⟩
 
 -- instance {m} [Functor m] [Iterator α m β] : Iterator (Iter (α := α) m β) m β where
@@ -59,20 +61,20 @@ def toIter (m) [Iterator α m β] (it : Iterator.α' α m) : Iter (α := α) m �
 --   wf := InvImage.wf (productiveIteratorWF ∘ Iter.inner ∘ ProductiveIteratorWF.inner) Productive.wf
 
 @[always_inline, inline]
-def Iter.stepH {α : Type u} {m : Type w → Type w'} {β : Type v} [Monad m]
-    [Iterator α m β] (it : Iter (α := α) m β) : m it.EncodedStep :=
+def Iter.stepH [Monad m]
+    [Iterator α α' m β] (it : Iter (α := α) m β) : m it.EncodedStep :=
   Iter.EncodedStep.ofInternal <$> Iterator.step it.inner
 
 @[always_inline, inline]
-def Iter.stepCont {α : Type u} {m : Type w → Type w'} {β : Type v} [Monad m]
-    [Iterator α m β] (it : Iter (α := α) m β) {γ} : ContT m γ it.Step :=
+def Iter.stepCont [Monad m]
+    [Iterator α α' m β] (it : Iter (α := α) m β) {γ} : ContT m γ it.Step :=
   fun h => it.stepH >>= (h ·.decode)
 
 @[always_inline, inline]
-def Iter.step {α β : Type u} (m : Type u → Type w) [Monad m]
-    [Iterator α m β] (it : Iter (α := α) m β) : m (Iter.Step it) :=
+def Iter.step {α' : Type u} {α β : Type w} (m : Type w → Type w) [Monad m]
+    [Iterator α α' m β] (it : Iter (α := α) m β) : m (Iter.Step it) :=
   Iter.EncodedStep.decode <$> it.stepH
 
 @[always_inline, inline]
-def Iter.terminationByFinite {α β m} [Iterator α m β] [Finite α m] (it : Iter (α := α) m β) : FiniteIteratorWF α m :=
+def Iter.terminationByFinite [Iterator α α' m β] [Finite α m] (it : Iter (α := α) m β) : FiniteIteratorWF α m :=
   finiteIteratorWF it.inner
