Iterator/Combinators/Take.lean
@@ -10,19 +10,18 @@ import Iterator.AbstractIteration
 This file provides the iterator combinator `Iter.take`.
 -/
 
-variable {α : Type u} {m : Type w → Type w'} {β : Type v}
+variable {α : Type w} {α' : Type u} {m : Type w → Type w'} {β : Type v}
 
 @[ext]
 structure Take (α : Type u) where
   remaining : Nat
   inner : α
 
-instance [Monad m] [Iterator α m β] : SimpleIterator (Take α) m β where
-  α' := Take (Iterator.α' α m)
-  β' := Iterator.β' α m
+instance [Monad m] [Iterator α α' m β] : SimpleIterator (Take α) (Take α') m β where
+  βInternal := Iterator.βInternal α m
   αEquiv := {
-    hom it := { inner := Iterator.αEquiv.hom it.inner, remaining := it.remaining }
-    inv it := { inner := Iterator.αEquiv.inv it.inner, remaining := it.remaining }
+    hom it := { inner := Iterator.αEquiv m |>.hom it.inner, remaining := it.remaining }
+    inv it := { inner := Iterator.αEquiv m |>.inv it.inner, remaining := it.remaining }
     hom_inv := by simp [Equiv.hom_inv]
     inv_hom := by simp [Equiv.inv_hom]
   }
@@ -62,24 +61,23 @@ _TODO_: prove `Productive`
 This combinator incurs an additional O(1) cost with each output of `it`.
 -/
 @[inline]
-def Iter.take [Iterator α m β] [Monad m] (n : Nat) (it : Iter (α := α) m β) :=
+def Iter.take [Iterator α α' m β] [Monad m] (n : Nat) (it : Iter (α := α) m β) :=
   toIter (α := Take α) m <| Take.mk n it.inner
 
-def Take.rel (m : Type w → Type w') [Monad m] [Iterator α m β] :
-    Iterator.α' (Take α) m → Iterator.α' (Take α) m → Prop :=
+def Take.rel (m : Type w → Type w') [Monad m] [Iterator α α' m β] : Take α → Take α → Prop :=
   InvImage (Prod.Lex Nat.lt_wfRel.rel ProductiveIteratorWF.lt)
     (fun it => (it.remaining, productiveIteratorWF (α := α) (m := m) it.inner))
 
-theorem Take.rel_of_remaining [Monad m] [Iterator α m β] {it it' : Iterator.α' (Take α) m}
+theorem Take.rel_of_remaining [Monad m] [Iterator α α' m β] {it it' : Take α}
     (h : it'.remaining < it.remaining) : Take.rel m it' it :=
   Prod.Lex.left _ _ h
 
-theorem Take.rel_of_inner [Monad m] [Iterator α m β] {remaining : Nat} {it it' : Iterator.α' α m}
+theorem Take.rel_of_inner [Monad m] [Iterator α α' m β] {remaining : Nat} {it it' : α}
     (h : (productiveIteratorWF (m := m) it').lt (productiveIteratorWF it)) :
     Take.rel m ⟨remaining, it'⟩ ⟨remaining, it⟩ :=
   Prod.Lex.right _ h
 
-instance [Monad m] [Iterator α m β] [Productive α m] : SimpleIterator.Finite (Take α) m where
+instance [Monad m] [Iterator α α' m β] [Productive α m] : SimpleIterator.Finite (Take α) m where
   rel := Take.rel m
   wf := by
     apply InvImage.wf
